backup

process/processes.v
@@ -1,5 +1,4 @@
 From mathcomp Require Import all_ssreflect.
-From elpi.apps Require Import derive.std.
 From SST Require Import aux.unscoped aux.expressions type.global tree.global tree.local. 
 Require Import List String Datatypes ZArith Relations Setoid Morphisms.
 Open Scope list_scope.
@@ -11,7 +10,6 @@ Require Import Coq.Arith.PeanoNat.
 Require Import JMeq.
 
 Section process.
-
 
 Inductive process : Type := 
   | p_var : fin -> process
@@ -26,7 +24,7 @@ Section process_ind_ref.
   Hypothesis P_var : forall n, P (p_var n).
   Hypothesis P_inact : P (p_inact).
   Hypothesis P_send : forall pt lb ex pr, P pr -> P (p_send pt lb ex pr).
-  Hypothesis P_recv : forall pt lb pr llb llp, Forall P llp -> P (p_recv pt lb pr llb llp).
+  Hypothesis P_recv : forall pt llb llp, Forall P llp -> P (p_recv pt llb llp).
   Hypothesis P_ite : forall e P1 P2, P P1 -> P P2 -> P (p_ite e P1 P2).
   Hypothesis P_rec : forall n pr, P pr -> P (p_rec n pr).
   
@@ -37,63 +35,48 @@ Section process_ind_ref.
     - apply (P_inact).
     - apply (P_send s n e p (process_ind_ref p)).
     - apply (P_recv).
-      - apply (process_ind_ref p). 
-      induction l as [ | c l IH].
-      clear process_ind_ref.
-      - intros. apply ForallR_nil.
-      - specialize(ForallR_cons P (fst c) (snd c) l); intros.
-        - generalize (process_ind_ref (snd c)). intros. 
-          specialize(H H0 IH); intros.
-          specialize(surjective_pairing c); intros.
-          replace c with (c.1, c.2). easy.
+      induction l0 as [ | c l0 IH].
+      clear process_ind_ref. 
+      - easy.
+      - apply (Forall_cons); intros. 
+        - generalize (process_ind_ref c); intros. apply H.
+        - apply IH.
     - apply (P_ite e p1 p2 (process_ind_ref p1) (process_ind_ref p2)).
     - apply (P_rec n p (process_ind_ref p)). 
   Qed.
 End process_ind_ref.
 
+Compute (length []) <> 0%nat.
 
-Section process_ind_ref.
-  Variable P : process -> Prop.
-  Hypothesis P_var : forall n, P (p_var n).
-  Hypothesis P_inact : P (p_inact).
-  Hypothesis P_send : forall pt lb ex pr, P pr -> P (p_send pt lb ex pr).
-  Hypothesis P_recv : forall pt lb pr llbp, ForallR P llbp -> P (p_recv pt lb pr llbp).
-  Hypothesis P_ite : forall e P1 P2, P P1 -> P P2 -> P (p_ite e P1 P2).
-  Hypothesis P_rec : forall n pr, P pr -> P (p_rec n pr).
+Inductive SSortedNList : list fin -> Prop :=
+  | sort1 : forall a, SSortedNList [a]
+  | sort2 : forall (z1 z2 : fin), forall l, le z1 z2 -> SSortedNList (z2 :: l) -> SSortedNList (z1 :: z2 :: l).
   
-  Fixpoint process_ind_ref p : P p.
-  Proof.
-    destruct p.
-    - apply (P_var n).
-    - apply (P_inact).
-    - apply (P_send s n e p (process_ind_ref p)).
-    - apply (P_recv).
-      - apply (process_ind_ref p). 
-      induction l as [ | c l IH].
-      clear process_ind_ref.
-      - intros. apply ForallR_nil.
-      - specialize(ForallR_cons P (fst c) (snd c) l); intros.
-        - generalize (process_ind_ref (snd c)). intros. 
-          specialize(H H0 IH); intros.
-          specialize(surjective_pairing c); intros.
-          replace c with (c.1, c.2). easy.
-    - apply (P_ite e p1 p2 (process_ind_ref p1) (process_ind_ref p2)).
-    - apply (P_rec n p (process_ind_ref p)). 
-  Qed.
-End process_ind_ref.
+Lemma test : not (SSortedNList []).
+Proof. 
+  intros. intuition.
+  inversion H.
+Qed.
 
+Inductive wtyped : process -> Prop := 
+  | wp_var : forall n, wtyped (p_var n)
+  | wp_inact : wtyped p_inact
+  | wp_send: forall pt lb ex pr, wtyped pr -> wtyped (p_send pt lb ex pr)
+  | wp_recv : forall pt llb llp, length llb = length llp -> SSortedNList llb -> List.Forall wtyped llp -> wtyped (p_recv pt llb llp)
+  | wp_ite : forall e P1 P2, wtyped P1 -> wtyped P2 -> wtyped (p_ite e P1 P2)
+  | wp_rec : forall n pr, wtyped pr -> wtyped (p_rec n pr).
 
 Fixpoint vars (P : process) : list fin :=
   match P with
     | p_var x => [x]
     | p_send p l e P' => vars P'
-    | p_recv p _ ct llbp => 
+    | p_recv p llb llp => 
        let fix next xs :=
          match xs with 
-          | (_,p)::ys => vars p ++ next ys
+          | p::ys => vars p ++ next ys
           | [] => []
          end
-       in next llbp ++ vars ct
+       in next llp
     | p_ite e p q => (vars p) ++ (vars q)
     | p_rec n p => n :: vars p
     | _ => []
@@ -104,44 +87,132 @@ Fixpoint rename_force (from : fin) (to : fin) (P : process) : process :=
   match P with 
     | p_var x => if Nat.eqb x from then p_var to else p_var x
     | p_send p l e P' => p_send p l e (rename_force from to P')
-    | p_recv p lb ct llbp => p_recv p lb (rename_force from to ct) (list_map (fun x => (fst x, rename_force from to (snd x))) llbp)
+    | p_recv p llb llp => p_recv p llb (list_map (rename_force from to) llp)
     | p_ite e p1 p2 => p_ite e (rename_force from to p1) (rename_force from to p2)
     | p_rec x P' => if Nat.eqb from x then P else p_rec x (rename_force from to P')
     | _ => P
   end. 
 
 
-Definition fresh_in (x : fin) (P : process) : Prop :=
-  let fix isin x lis :=
-    match lis with
-      | y::ys => x <> y /\ isin x ys
-      | _ => True
-    end
-  in isin x (vars P).
+Fixpoint fresh_in (x : fin) (P : process) : Prop :=
+  match P with 
+    | p_inact => True 
+    | p_var n => x <> n
+    | p_send p l e P'  => fresh_in x P'
+    | p_recv p llb llp => 
+        let fix next_lis lis := 
+          match lis with 
+            | [] => True 
+            | y::ys => fresh_in x y /\ next_lis ys 
+          end
+        in next_lis llp
+    | p_ite e p1 p2 => fresh_in x p1 /\ fresh_in x p2
+    | p_rec y P' => x <> y /\ fresh_in x P'
+  end.   
+
+Lemma not_vars_implies_fresh_list : forall x pt llb llp, (Forall (fun P : process => ~ In x (vars P) -> fresh_in x P) llp) -> 
+               ~ In x (vars (p_recv pt llb llp)) -> fresh_in x (p_recv pt llb llp).
+Proof.
+  intros x pt llb llp. induction llp; intros; try easy.
+  specialize(Forall_cons_iff (fun P : process => ~ In x (vars P) -> fresh_in x P) a llp); intros. destruct H1.
+  specialize(H1 H); intros. clear H2. destruct H1.
+  specialize(IHllp H2); intros. clear H2.
+  simpl in H0. specialize(in_app_iff (vars a) (vars (p_recv pt llb llp)) x); intros. destruct H2.
+  specialize(contra_not H3); intros. clear H2 H3.
+  specialize(H4 H0); intros. 
+  specialize(Decidable.not_or (In x (vars a)) (In x (vars (p_recv pt llb llp))) H4); intros. destruct H2.
+  specialize(H1 H2); intros.
+  specialize(IHllp H3); intros.
+  simpl. split. easy. easy.
+Qed.
+
+Lemma not_vars_implies_fresh : forall x P, not (In x (vars P)) -> fresh_in x P.
+Proof.
+  intros x P. induction P using process_ind_ref; intros; try easy.
+  - simpl in *. specialize(Decidable.not_or (n = x) False H); intros. destruct H0. easy.
+  - simpl in H. specialize(IHP H); intros. simpl. easy.
+  - apply not_vars_implies_fresh_list. easy. easy.
+  - simpl. simpl in H. 
+    specialize(in_app_iff (vars P1) (vars P2) x); intros. destruct H0.
+    specialize(contra_not H1); intros. specialize(H2 H); intros.
+    specialize(Decidable.not_or (In x (vars P1)) (In x (vars P2)) H2); intros. destruct H3.
+    specialize(IHP1 H3); intros. specialize(IHP2 H4); intros; try easy.
+  - simpl. simpl in H. specialize(Decidable.not_or (n = x) (In x (vars P)) H); intros. destruct H0.
+    specialize(IHP H1); intros. easy.
+Qed.
+
+Fixpoint mx_list (lis : list fin) : fin :=
+  match lis with 
+    | x::xs => max x (mx_list xs)
+    | []    => 0
+  end.
+
+Search (Forall).
+
+Lemma succ_max_not_in_list : forall lis, not (In (mx_list lis + 1) lis).
+Admitted.
+
+Lemma exists_not_in_var : forall P, exists k, not (In k (vars P)).
+Proof.
+  intros. exists (mx_list (vars P) +1).
+  specialize(succ_max_not_in_list (vars P)). easy.
+Qed.
+
+Lemma exists_fresh : forall P, exists k, fresh_in k P.
+Proof.
+    intros.
+    specialize(exists_not_in_var P); intros.
+    destruct H.
+    specialize(not_vars_implies_fresh x P H); intros.
+    exists x. easy.
+Qed.
 
 Lemma freshness_in_rec : forall (x y : fin) (P : process), fresh_in y (p_rec x P) -> (y <> x).
 Proof.
   intros x y P.
-  unfold fresh_in. unfold vars.
-  easy.
+  simpl. easy.
 Qed.
   
+Lemma freshness_in_var : forall n m, fresh_in n (p_var m) -> n <> m.
+Proof.
+  intros. 
+  unfold fresh_in in H. unfold vars in H. easy.
+Qed.
+
+Lemma freshness_in_send : forall m pt lb ex P, fresh_in m (p_send pt lb ex P) -> fresh_in m P.
+Proof.
+  intros. easy.
+Qed.
+
+Lemma freshness_in_recv : forall m pt llb llp, fresh_in m (p_recv pt llb llp) -> List.Forall (fresh_in m) llp.
+Proof.
+  intros m pt llb llp. induction llp.
+  - intros. easy.
+  - intros. specialize(Forall_cons_iff (fresh_in m) a llp); intros. destruct H0.
+    apply H1. split. simpl in H. destruct H. easy.
+    assert(fresh_in m (p_recv pt llb llp)).
+    {
+      simpl.
+      simpl in H. destruct H. easy.
+    }
+    specialize(IHllp H2); intros. easy.
+Qed.
+
 Definition p_rename (from : fin) (to : fin) (P : process) (Q : process) : Prop := 
   rename_force from to P = Q.
   
 Section alphaP.
 
- 
+
+
+
 Inductive alphaP : relation process :=
   | a_inact : alphaP (p_inact) (p_inact)
   | a_var : forall n, alphaP (p_var n) (p_var n)
   | a_send : forall p l e P P', alphaP P P' -> alphaP (p_send p l e P) (p_send p l e P')
-  | a_recv : forall p llb xs ys lb x y, length llb = length xs -> length llb = length ys -> alphaP x y -> List.Forall2 alphaP xs ys -> alphaP (p_recv p lb x (zip llb xs)) (p_recv p lb y (zip llb ys))
+  | a_recv : forall p llb xs ys, List.Forall2 alphaP xs ys -> alphaP (p_recv p llb xs) (p_recv p llb ys)
   | a_ite  : forall e P1 P2 Q1 Q2, alphaP P1 Q1 -> alphaP P2 Q2 -> alphaP (p_ite e P1 P2) (p_ite e Q1 Q2)
-  | a_recl  : forall x y P Q, fresh_in y (p_rec x P) -> p_rename x y P Q -> alphaP P Q -> alphaP (p_rec x P) (p_rec y Q)
-  | a_recr  : forall x y P Q, fresh_in x (p_rec y Q) -> p_rename y x Q P -> alphaP P Q -> alphaP (p_rec x P) (p_rec y Q)
-  | a_rec2  : forall x P Q, alphaP P Q -> alphaP (p_rec x P) (p_rec x Q).
-
+  | a_rec  : forall x y z P Q, fresh_in z (p_rec x P) -> fresh_in z (p_rec y Q) -> alphaP (rename_force x z P) (rename_force y z Q) -> alphaP (p_rec x P) (p_rec y Q).
 
 Definition Forall2_mono {X Y} {R T : X -> Y -> Prop} (HRT : forall x y, R x y -> T x y) :
       forall l m, Forall2 R l m -> Forall2 T l m :=
@@ -157,23 +228,24 @@ Section alphaP_ind_ref.
   Hypothesis P_inact : P p_inact p_inact.
   Hypothesis P_var  : forall n, P (p_var n) (p_var n).
   Hypothesis P_send : forall p l e P1 P2, P P1 P2 -> P (p_send p l e P1) (p_send p l e P2).
-  Hypothesis P_recv : forall p lb x y llb xs ys, length llb = length xs -> length llb = length ys -> P x y 
-                      -> List.Forall2 P xs ys -> P (p_recv p lb x (zip llb xs)) (p_recv p lb y (zip llb ys)).
+  Hypothesis P_recv : forall p llb xs ys, List.Forall2 P xs ys -> P (p_recv p llb xs) (p_recv p llb ys).
   Hypothesis P_ite  : forall e P1 P2 Q1 Q2, P P1 Q1 -> P P2 Q2 -> P (p_ite e P1 P2) (p_ite e Q1 Q2).
-  Hypothesis P_recl : forall x y P1 P2, fresh_in y (p_rec x P1) -> p_rename x y P1 P2 -> P P1 P2 -> P (p_rec x P1) (p_rec y P2).
-  Hypothesis P_recr : forall x y P1 P2, fresh_in x (p_rec y P2) -> p_rename y x P2 P1 -> P P1 P2 -> P (p_rec x P1) (p_rec y P2).
-  Hypothesis P_recn : forall x P1 P2, P P1 P2 -> P (p_rec x P1) (p_rec x P2). 
+  Hypothesis P_rec  : forall x y z P1 P2, fresh_in z (p_rec x P1) -> fresh_in z (p_rec y P2) -> P (rename_force x z P1) (rename_force y z P2) -> P (p_rec x P1) (p_rec y P2).
+(*   Hypothesis P_recl : forall x y P1 P2, fresh_in y (p_rec x P1) -> alphaP (rename_force x y P1) P2 -> P (p_rec x P1) (p_rec y P2).
+  Hypothesis P_recr : forall x y P1 P2, fresh_in x (p_rec y P2) -> alphaP (rename_force y x P2) P1  -> P (p_rec x P1) (p_rec y P2).
+  Hypothesis P_recn : forall x P1 P2, P P1 P2 -> P (p_rec x P1) (p_rec x P2).  *)
 
   Fixpoint alphaP_ind_ref (P1 P2 : process) (a : alphaP P1 P2) {struct a} : P P1 P2 :=
     match a with 
       | a_inact => P_inact
       | a_var n => P_var n
       | a_send p l e P1 P2 H => P_send p l e P1 P2 (alphaP_ind_ref P1 P2 H) 
-      | a_recv p llb xs ys lb x y Hlx Hly Ha La => P_recv p lb x y llb xs ys Hlx Hly (alphaP_ind_ref x y Ha) (Forall2_mono alphaP_ind_ref xs ys La)
+      | a_recv p llb xs ys La => P_recv p llb xs ys (Forall2_mono alphaP_ind_ref xs ys La)
       | a_ite e P1 P2 Q1 Q2 H1 H2 => P_ite e P1 P2 Q1 Q2 (alphaP_ind_ref P1 Q1 H1) (alphaP_ind_ref P2 Q2 H2)
-      | a_recl x y P1 P2 Hfy Hr Ha => P_recl x y P1 P2 Hfy Hr (alphaP_ind_ref P1 P2 Ha)
-      | a_recr x y P1 P2 Hfy Hr Ha => P_recr x y P1 P2 Hfy Hr (alphaP_ind_ref P1 P2 Ha)
-      | a_rec2 x P1 P2 Ha => P_recn x P1 P2 (alphaP_ind_ref P1 P2 Ha)
+      | a_rec x y z P1 P2 Hfx Hfy Hr => P_rec x y z P1 P2 Hfx Hfy (alphaP_ind_ref (rename_force x z P1) (rename_force y z P2) Hr)
+(*       | a_recl x y P1 P2 Hfy Hr => P_recl x y P1 P2 Hfy Hr
+      | a_recr x y P1 P2 Hfy Hr => P_recr x y P1 P2 Hfy Hr
+      | a_rec2 x P1 P2 Ha => P_recn x P1 P2 (alphaP_ind_ref P1 P2 Ha) *)
     end.
 
 End alphaP_ind_ref.
@@ -199,32 +271,26 @@ Proof.
     replace a with (a.1,a.2). easy.
 Qed.
 
-Lemma refl_alphaP : forall P, alphaP P P.
+Lemma refl_alphaP_helper : forall llp, Forall wtyped llp -> Forall (fun P : process => wtyped P -> alphaP P P) llp -> Forall2 alphaP llp llp.
 Proof.
-  intros. 
-  induction P using process_ind_ref.
-  - specialize(a_var n); intros; try easy.
-  - specialize(a_inact); intros; try easy.
-  - specialize(a_send pt lb ex P P IHP); intros; try easy.
-  - specialize(a_recv); intros.
-    induction llbp.
-      - specialize(H0 pt [] [] [] lb P P); intros. 
-        specialize(H0 (Logic.eq_refl (length [])) (Logic.eq_refl (length [])) IHP); intros.
-        assert(Forall2 alphaP [] []). { easy. }
-        specialize(H0 H1); intros; try easy.
-        specialize(H0 pt (list_map fst (a::llbp)) (list_map snd (a::llbp)) (list_map snd (a::llbp)) lb P P); intros.
-        specialize((list_fst_snd_len (a::llbp))); intros.
-        specialize(H0 H1 H1 IHP); intros.
-        specialize(unzip_zip (a::llbp)); intros. 
-        replace (zip (list_map fst (a :: llbp)) (list_map snd (a :: llbp))) with (a::llbp) in H0.
-        clear H1 H2.
-        
-        
-        
-        specialize( IHP); intros.
-      -  
+  intro llp.
+  induction llp.
+  intros. easy.
+  intros. specialize(Forall_cons_iff); intros.
+  specialize(H1 process wtyped a llp); intros. destruct H1.
+  specialize(H1 H); intros. clear H H2. destruct H1.
+  specialize(Forall_cons_iff); intros.
+  specialize(H2 process (fun P : process => wtyped P -> alphaP P P) a llp); intros. destruct H2.
+  specialize(H2 H0); intros. clear H0 H3. destruct H2.
+  specialize(IHllp H1 H2); intros.
+  specialize(H0 H); intros. clear H H1.
+  
+  specialize(Forall2_cons_iff); intros. 
+  specialize(H process process alphaP a a llp llp); intros. destruct H.
+  apply H1. split. easy. easy.
+Qed.
 
-Lemma sym_alphaP : forall P Q, alphaP P Q -> alphaP Q P.
+Lemma alphaP_sym : forall P Q, alphaP P Q -> alphaP Q P.
 Proof.
   intros.
   induction H using alphaP_ind_ref; intros; try easy.
@@ -233,18 +299,452 @@ Proof.
   - specialize(a_send p l e P2 P1 IHalphaP); intros. easy.
   - assert(Forall2 alphaP ys xs).
     {
-      specialize(Forall2_flip H1); intros.
-      simpl in H2. easy.
+      specialize(Forall2_flip H); intros.
+      simpl in H0. easy.
     }
-    specialize(a_recv p llb ys xs lb y x H0 H IHalphaP H2); intros. easy.
+    specialize(a_recv p llb ys xs H0); intros. easy.
   - specialize(a_ite e Q1 Q2 P1 P2 IHalphaP IHalphaP0); intros. easy.
-  - specialize(a_recr y x P2 P1 H H0 IHalphaP); intros. easy.
-  - specialize(a_recl y x P2 P1 H H0 IHalphaP); intros. easy.
-  - specialize(a_rec2 x P2 P1 IHalphaP); intros. easy.
+  - specialize(a_rec y x z P2 P1 H0 H IHalphaP); intros. easy.
+Qed.
+
+Lemma rename_trans : forall x1 x2 x3 P, rename_force x2 x3 (rename_force x1 x2 P) = rename_force x1 x3 P.
+Admitted.
+
+Lemma strong_ind (P : nat -> Prop) :
+  (forall m, (forall k : nat, lt k m -> P k) -> P m) ->
+    forall n, P n.
+Proof.
+  intros H n; enough (H0: forall p, le p n -> P p).
+    - apply H0, Nat.le_refl.
+    - induction n.
+      + intros. apply H. inversion H0. easy.
+      + intros. apply H. intros. apply IHn.  inversion H0. 
+        * rewrite H2 in H1. apply PeanoNat.lt_n_Sm_le in H1. assumption.
+        * specialize (PeanoNat.Nat.lt_le_trans k p n H1 H3). apply PeanoNat.Nat.lt_le_incl.
+Qed.
+
+Fixpoint process_size (P : process) : fin := 
+  match P with 
+    | p_var n => 0 
+    | p_inact => 0
+    | p_send pt lb e p => 1 + process_size p 
+    | p_recv pt llb lp => 
+      let fix mx_siz lis := 
+        match lis with 
+          | x::xs => max (process_size x) (mx_siz xs)
+          | [] => 0
+        end
+      in 1 + mx_siz lp
+    | p_ite e p1 p2 => 1 + max (process_size p1) (process_size p2)
+    | p_rec n p => 1 + (process_size p)
+  end.
+
+Lemma psize_exists : forall P, exists n, process_size P = n.
+Proof.
+  intro P. 
+  exists (process_size P). easy.
+Qed.
+
+Lemma size_cons_rename : forall m n P, process_size P = process_size (rename_force m n P).
+Proof.
+  intros. induction P using process_ind_ref; intros; try easy.
+  - simpl. case_eq (Nat.eqb n0 m); intros. easy. easy.
+  - simpl. replace (process_size P) with (process_size (rename_force m n P)). easy.
+  - induction llp. 
+    - simpl. easy.
+    - simpl. specialize(Forall_cons_iff (fun P : process =>
+       process_size P = process_size (rename_force m n P)) a llp); intros. destruct H0.
+      specialize(H0 H); intros. clear H1. destruct H0. 
+      replace (process_size (rename_force m n a)) with (process_size a).
+      specialize(IHllp H1); intros.
+      simpl in IHllp. specialize(eq_add_S ((fix mx_siz (lis : seq process) : fin :=
+           match lis with
+           | [] => 0
+           | (x :: xs)%list => Init.Nat.max (process_size x) (mx_siz xs)
+           end) llp) ((fix mx_siz (lis : seq process) : fin :=
+           match lis with
+           | [] => 0
+           | (x :: xs)%list => Init.Nat.max (process_size x) (mx_siz xs)
+           end) (list_map (rename_force m n) llp)) IHllp); intros.
+      replace ((fix mx_siz (lis : seq process) : fin :=
+      match lis with
+      | [] => 0
+      | (x :: xs)%list => Init.Nat.max (process_size x) (mx_siz xs)
+      end) (list_map (rename_force m n) llp)) with ((fix mx_siz (lis : seq process) : fin :=
+      match lis with
+      | [] => 0
+      | (x :: xs)%list => Init.Nat.max (process_size x) (mx_siz xs)
+      end) llp). easy.
+  - simpl. 
+    replace (process_size P1) with (process_size (rename_force m n P1)).
+    replace (process_size P2) with (process_size (rename_force m n P2)). easy.
+  - simpl. case_eq (Nat.eqb m n0); intros.
+    - simpl. easy.
+    - simpl. replace (process_size P) with (process_size (rename_force m n P)). easy.
+Qed.
+
+Lemma alphaP_refl : forall P, alphaP P P.
+Proof.
+  intro P.
+  specialize(psize_exists P); intros.
+  destruct H. revert H. revert P. 
+  induction x using strong_ind.
+  destruct P. intros; try easy.
+  - apply a_var.
+  - intros. apply a_inact.
+  - intros. apply a_send. simpl in H0.
+    specialize(H (process_size P)); intros. 
+    admit.
+  - intros. apply a_recv. simpl in H0.
+    admit.
+  - admit.
+  - admit.
+Admitted.
+  
+
+Lemma alphaP_refl_rename : forall m n P, alphaP P P -> fresh_in n P -> alphaP (rename_force m n P) (rename_force m n P).
+Proof.
+  intros m n P. 
+  induction P using process_ind_ref; intros; try easy.
+  - simpl.
+    case_eq (Nat.eqb n0 m); intros.
+     - replace (n0 =? m)%nat with true.
+       admit.
+     - easy.
+  - simpl. inversion H. subst.
+    specialize(IHP H2); intros.
+    apply a_send. simpl in H0. apply IHP. easy.
+  - admit.
+  - simpl. inversion H. subst. 
+    simpl in H0. destruct H0.
+    specialize(IHP1 H3 H0); intros. specialize(IHP2 H7 H1); intros.
+    apply a_ite. easy. easy.
+  - simpl.
+    case_eq (Nat.eqb m n0); intros.
+    - easy.
+    - 
+      
+      
+  
+  Admitted.
+
+Lemma alphaP_refl : forall P, wtyped P -> alphaP P P.
+Proof.
+  intros. 
+  induction P using process_ind_ref.
+  - specialize(a_var n); intros; try easy.
+  - specialize(a_inact); intros; try easy.
+  - inversion H.
+  
+    specialize(IHP H1); intros.
+    specialize(a_send pt lb ex P P IHP); intros; try easy.
+    
+  - specialize(a_recv); intros.
+    inversion H. subst.
+    specialize(H1 pt llb llp llp H5 H5); intros.
+    specialize(refl_alphaP_helper llp H7 H0); intros.
+    specialize(H1 H2); intros. easy.
+    
+  - specialize(a_ite e P1 P2 P1 P2); intros.
+    inversion H. subst.
+    specialize(IHP1 H3); intros.
+    specialize(IHP2 H5); intros.
+    specialize(H0 IHP1 IHP2); intros; try easy.
+  
+  - inversion H. subst. specialize(IHP H1); intros.
+    specialize(exists_fresh (p_rec n P)); intros.
+    destruct H0.
+    specialize(a_rec n n x P P H0 H0); intros.
+    specialize(alphaP_refl_rename n x P IHP); intros. simpl in H0. destruct H0.
+    specialize(H3 H4); intros.
+    specialize(H2 H3); easy. 
+Qed.
+
+  
+
+
+Lemma inv_alphaP_inact : forall P, alphaP P p_inact -> P = p_inact.
+Proof.
+  intros. inversion H. easy.
+Qed.
+
+Lemma inv_alphaP_var : forall P n, alphaP P (p_var n) -> P = p_var n.
+Proof.
+  intros. inversion H. easy.
+Qed. 
+
+Lemma inv_alphaP_send : forall P P' p l e, alphaP P (p_send p l e P') 
+  -> exists Q, P = p_send p l e Q /\ alphaP Q P'.
+Proof.
+  intros. inversion H. exists P0. 
+  split. easy. easy.
+Qed.
+
+Lemma positive_list_length_dst {A} : forall (xs : list A) n, length xs = S(n) -> exists y ys, y::ys = xs.
+Proof.
+  intros.
+  induction xs. easy.
+  exists a. exists xs. easy.
+Qed.
+
+Lemma forall2_alphaP_sym : forall xs ys, List.Forall2 alphaP xs ys -> List.Forall2 alphaP ys xs.
+Proof.
+  intro xs. induction xs.
+  intros. 
+  specialize(Forall2_length H); intros. simpl in *. 
+  specialize(length_zero_iff_nil ys); intros.  destruct H1.
+  specialize(H1 (esym H0)). subst. easy.
+  intros.
+  specialize(Forall2_length H); intros. simpl in *.
+  specialize(positive_list_length_dst ys (length xs) (esym H0)); intros.
+  destruct H1. destruct H1. subst. simpl in *.
+  specialize(Forall2_cons_iff alphaP a x xs x0); intros. destruct H1. 
+  specialize(H1 H); intros.
+  destruct H1.
+  specialize(IHxs x0 H3); intros.
+  specialize(alphaP_sym a x H1); intros. 
+  specialize(Forall2_cons x a H4 IHxs); intros. easy.
+Qed.
+
+Lemma inv_alphaP_recv : forall P pt llb llp, alphaP P (p_recv pt llb llp) -> exists Q, P = p_recv pt llb Q /\ List.Forall2 alphaP llp Q /\ length llb = length Q /\ length llb = length llp.
+Proof.
+  intros. inversion H. exists xs. 
+  split. easy. split. subst.
+  specialize(forall2_alphaP_sym xs llp H6); intros. easy.
+  easy.
+Qed.
+
+Lemma inv_alphaP_ite : forall P e P1 P2, alphaP P (p_ite e P1 P2) -> exists Q1 Q2, P = p_ite e Q1 Q2 /\ alphaP P1 Q1 /\ alphaP P2 Q2.
+Proof.
+  intros. inversion H. subst. exists P0. exists P3. split. easy.
+  split. 
+  specialize(alphaP_sym P0 P1 H3); intros; try easy.
+  specialize(alphaP_sym P3 P2 H5); intros; try easy.
+Qed.
+
+Lemma list_renaming_invariance : forall llp n, Forall (fun P : process => forall n : fin, rename_force n n P = P) llp -> (list_map (rename_force n n) llp) = llp.
+Proof.
+  intro llp. induction llp.
+  intros. easy. 
+  specialize(Forall_cons_iff (fun P : process => forall n : fin, rename_force n n P = P) a llp); intros.
+  destruct H. specialize(H H0); intros. clear H0 H1. destruct H.
+  simpl.
+  specialize(IHllp n H0); intros. 
+  replace (list_map (rename_force n n) llp) with llp.
+  specialize(H n); intros.
+  replace (rename_force n n a) with a. easy.
+Qed.
+
+Lemma renaming_invariance : forall P n, rename_force n n P = P.
+Proof.
+  intro P. induction P using process_ind_ref; intros; try easy.
+  - case_eq (Nat.eqb n n0); intros.
+    - simpl. replace (n =? n0)%nat with true. 
+      specialize(Nat.eqb_eq n n0); intros. destruct H0. specialize(H0 H); intros. subst. easy.
+    - simpl. replace (n =? n0)%nat with false. easy.
+  - simpl. specialize(IHP n); intros. replace (rename_force n n P) with P. easy.
+  - simpl. specialize(list_renaming_invariance llp n H); intros. 
+    replace (list_map (rename_force n n) llp) with llp.
+    easy.
+  - simpl. specialize(IHP1 n); intros. specialize(IHP2 n); intros.
+    replace (rename_force n n P1) with P1. replace (rename_force n n P2) with P2. easy.
+  - simpl. case_eq(Nat.eqb n0 n); intros.
+    - easy.
+    - simpl. specialize(IHP n0); intros.
+      replace (rename_force n0 n0 P) with P. easy.
+Qed.
+
+Lemma inv_alphaP_rec : forall P n Q, alphaP P (p_rec n Q) -> exists m z Q', P = p_rec m Q' /\ 
+        (alphaP (rename_force n z Q) (rename_force m z Q') /\ fresh_in z (p_rec n Q) /\ fresh_in z (p_rec m Q')).
+Proof.
+  intros. inversion H.
+  - subst. exists x. exists z. exists P0. split. easy. split. 
+    specialize(alphaP_sym (rename_force x z P0) (rename_force n z Q) H5); intros. easy. easy.
 Qed.
 
 
+(* 
+Lemma renaming_reversal_list : forall n m x llp, Forall (fresh_in m) llp -> Forall2 alphaP (list_map (rename_force n m) llp) x -> Forall
+      (fun P : process =>
+       forall (Q : process) (n m : fin),
+       alphaP (rename_force n m P) Q ->
+       fresh_in m P -> alphaP (rename_force m n Q) P) llp -> Forall2 alphaP (list_map (rename_force m n) x) llp.
+Proof.
+  intros n m x llp. revert x.
+  induction llp.
+  intros. 
+  simpl in H0. 
+  specialize(Forall2_length H0); intros. simpl in H2.
+  specialize(length_zero_iff_nil x); intros. destruct H3.
+  specialize(H3 (esym H2)); intros. subst. easy.
+  intros.
+  specialize(Forall_cons_iff (fresh_in m) a llp); intros. destruct H2.
+  specialize(H2 H); intros. clear H3. destruct H2.
+  specialize(Forall2_length H0); intros. simpl in H4.
+  specialize(positive_list_length_dst x (length (list_map (rename_force n m) llp))); intro.
+  specialize(H5 (esym H4)). destruct H5. destruct H5. subst. 
+  specialize(Forall2_cons_iff alphaP (rename_force n m a) x0 (list_map (rename_force n m) llp) x1); intros. destruct H5.
+  simpl in H0. 
+  specialize(H5 H0); intros. destruct H5. clear H6.
+  simpl in IHllp.
+  specialize(IHllp x1 H3 H7); intros.
+  specialize(Forall_cons_iff (fun P : process =>
+        forall (Q : process) (n m : fin),
+        alphaP (rename_force n m P) Q ->
+        fresh_in m P -> alphaP (rename_force m n Q) P) a llp); intros. 
+  destruct H6. specialize(H6 H1); intros. clear H7 H8. destruct H6.
+  specialize(IHllp H7); intros.       
+  specialize(H6 x0 n m H5 H2); intros.
+  simpl.
+  clear H H0 H1 H2 H3 H4 H5 H7.
+  specialize(Forall2_cons_iff alphaP (rename_force m n x0) a (list_map (rename_force m n) x1) llp); intros.
+  destruct H. simpl in H0. apply H0. clear H0 H. split.
+  easy. easy.
+Qed.
 
+Lemma renaming_reversal_alphaP : forall P Q n m, alphaP (rename_force n m P) Q -> fresh_in m P -> alphaP (rename_force m n Q) P.
+Proof.
+  intro P. induction P using process_ind_ref; intros; try easy.
+  - simpl in H.
+    case_eq(Nat.eqb n n0); intros.
+    - replace (n =? n0)%nat with true in H.
+      specialize(inv_alphaP_var Q m (alphaP_sym (p_var m) Q H)); intros. subst.
+      simpl. 
+      specialize(Nat.eqb_refl m); intros.
+      replace (m =? m)%nat with true.
+      specialize(Nat.eqb_eq n n0); intros. destruct H3. specialize(H3 H1). subst.
+      specialize(alphaP_refl (p_var n0)); intros; try easy.
+      specialize(wp_var n0); intros.
+      specialize(H3 H5); easy.
+    - replace (n =? n0)%nat with false in H. 
+      specialize(inv_alphaP_var Q n (alphaP_sym (p_var n) Q H)); intros. subst.
+      simpl. specialize(freshness_in_var m n H0); intros.
+      specialize(Nat.eqb_neq n m); intros. destruct H3.
+      specialize(nesym H2); intros.
+      specialize(H4 H5); intros. replace (n =? m)%nat with false. 
+      apply (a_var n).
+    - simpl in H. specialize(inv_alphaP_inact Q (alphaP_sym p_inact Q H)); intros.
+      subst. simpl. apply a_inact.
+    - specialize(freshness_in_send m pt lb ex P H0); intros.
+      simpl in H. specialize(inv_alphaP_send Q (rename_force n m P) pt lb ex); intros.
+      specialize(H2 (alphaP_sym (p_send pt lb ex (rename_force n m P)) Q H)); intros. 
+      destruct H2. destruct H2. subst.
+      specialize(IHP x n m (alphaP_sym x (rename_force n m P) H3) H1); intros.
+      simpl. 
+      specialize(a_send pt lb ex (rename_force m n x) P IHP); intros. easy.
+    - simpl in *. specialize(inv_alphaP_recv Q pt llb (list_map (rename_force n m) llp)); intros.
+      specialize(H2 (alphaP_sym (p_recv pt llb (list_map (rename_force n m) llp)) Q H0)); intros.
+      destruct H2. destruct H2. destruct H3. destruct H4.
+      subst. specialize(freshness_in_recv m pt llb llp H1); intros.
+      simpl.
+      specialize(renaming_reversal_list n m x llp H2 H3 H); intros.
+      specialize(a_recv pt llb (list_map (rename_force m n) x) llp); intros.
+      specialize(map_length (rename_force m n) x); intros. 
+      specialize(map_length (rename_force n m) llp); intros.
+      specialize(eq_trans H5 H9); intros.
+      specialize(eq_trans H4 (esym H8)); intros.
+      specialize(H7 H11 H10 H6); intros. easy.
+    - simpl in H.
+      specialize(inv_alphaP_ite Q e (rename_force n m P1) (rename_force n m P2)); intros.
+      specialize(alphaP_sym (p_ite e (rename_force n m P1) (rename_force n m P2)) Q H); intros.
+      specialize(H1 H2); intros. destruct H1. destruct H1. destruct H1. destruct H3.
+      inversion H0. subst.
+      specialize(IHP1 x n m H3 H5); intros.
+      specialize(IHP2 x0 n m H4 H6); intros.
+      simpl. 
+      specialize(a_ite e (rename_force m n x) (rename_force m n x0) P1 P2 IHP1 IHP2); intros. easy.
+    - simpl in H.
+      case_eq (Nat.eqb n0 n); intros. replace (n0 =? n)%nat with true in H.
+      specialize(inv_alphaP_rec Q n P (alphaP_sym (p_rec n P) Q H)); intros.
+      destruct H2. destruct H2. 
+      destruct H2. destruct H2. destruct H3. subst.
+      simpl in H0. destruct H0. simpl in H4. destruct H4. specialize(IHP x0 n x H3 H5); intros.
+      simpl.
+       - case_eq (Nat.eqb m x); intros. apply (alphaP_sym (p_rec n P) (p_rec x x0) H).
+       - specialize(a_recr); intros. 
+      
+      
+      
+      
+Admitted. 
+    *)
+    
+Lemma wtyped_through_fresh : forall P x z, wtyped P -> fresh_in z P -> wtyped (rename_force x z P).
+Admitted.
+
+Lemma wtyped_alphaP_helper : forall llp x, Forall
+      (fun P : process => forall Q : process, alphaP P Q -> wtyped P -> wtyped Q)
+      llp -> Forall2 alphaP llp x -> Forall wtyped llp -> Forall wtyped x.
+Proof.
+  intro llp. induction llp.
+  intros. 
+  - specialize(Forall2_length H0); intros. simpl in *.
+    specialize(length_zero_iff_nil x); intros. destruct H3.
+    specialize(H3 (esym H2)); intros. subst. easy.
+  - intros.
+    specialize(Forall2_length H0); intros. simpl in *.
+    specialize(positive_list_length_dst x (length llp) (esym H2)); intros.
+    destruct H3. destruct H3. subst.
+    specialize(IHllp x1); intros.
+    specialize(Forall_cons_iff (fun P : process => forall Q : process, alphaP P Q -> wtyped P -> wtyped Q) a llp); intros.
+    destruct H3. specialize(H3 H); intros. clear H4.
+    destruct H3.
+    specialize(IHllp H4); intros.
+    specialize(Forall2_cons_iff alphaP a x0 llp x1); intros. destruct H5.
+    specialize(H5 H0); intros. clear H6.
+    destruct H5.
+    specialize(Forall_cons_iff wtyped a llp); intros. destruct H7. clear H8. 
+    specialize(H7 H1); intros. destruct H7.
+    specialize(IHllp H6 H8); intros.
+    specialize(H3 x0 H5 H7); intros.
+    specialize(Forall_cons x0 H3 IHllp); intros. easy.
+Qed.
+
+Lemma wtyped_alphaP : forall P Q, alphaP P Q -> wtyped P -> wtyped Q.
+Proof.
+  intro P. induction P using process_ind_ref; intros; try easy.
+  - specialize(inv_alphaP_var Q n); intros. 
+    specialize(alphaP_sym (p_var n) Q H); intros. 
+    specialize(H1 H2); intros; try easy. subst. easy.
+  - specialize(inv_alphaP_inact Q); intros.
+    specialize(alphaP_sym p_inact Q H); intros. 
+    specialize(H1 H2); intros; try easy. subst. easy. 
+  - specialize(inv_alphaP_send Q P pt lb ex); intros.
+    specialize(alphaP_sym (p_send pt lb ex P) Q H); intros. 
+    specialize(H1 H2); intros. destruct H1. destruct H1. subst. 
+    specialize(alphaP_sym x P H3); intros.
+    specialize(IHP x H1); intros.
+    inversion H0. subst. 
+    specialize(IHP H5); intros.
+    apply (wp_send pt lb ex x). easy.
+  - specialize(inv_alphaP_recv Q pt llb llp); intros.
+    specialize(alphaP_sym (p_recv pt llb llp) Q H0); intros.
+    specialize(H2 H3); intros. 
+    destruct H2. destruct H2. destruct H4. destruct H5.
+    inversion H1; subst.
+    specialize(wp_recv pt llb x H5 H11); intros.
+    apply H2.
+    clear H0 H1 H5 H6 H10 H11 H2.
+    specialize(wtyped_alphaP_helper llp x H H4 H12); intros.
+    easy.
+  - specialize(inv_alphaP_ite Q e P1 P2 (alphaP_sym (p_ite e P1 P2) Q H)); intros.
+    destruct H1. destruct H1. destruct H1. destruct H2. subst.
+    inversion H0. subst.
+    specialize(IHP1 x H2 H5); intros.
+    specialize(IHP2 x0 H3 H7); intros.
+    specialize(wp_ite e x x0 IHP1 IHP2); intros. easy.
+  - specialize(inv_alphaP_rec Q n P (alphaP_sym (p_rec n P) Q H)); intros.
+    destruct H1. destruct H1. destruct H1. destruct H1. destruct H2. destruct H3.
+    inversion H0. subst. 
+    specialize(wtyped_through_fresh x1); intros.
+    
+Admitted.    
+    
+    
+    
+    
+
+(* 
 Lemma alphaP_inv_send : forall P P' p l e, alphaP P (p_send p l e P') 
   -> exists Q, P = p_send p l e Q /\ alphaP Q P'.
 Proof.
@@ -279,17 +779,13 @@ Proof.
   split. easy. split. 
   admit.
   admit.
-Admitted.
+Admitted. *)
      
 
 Inductive multi {X : Type} (R : relation X) : relation X :=
-  | multi_refl : forall (x : X), multi R x x
+  | multi_refl : forall (x : X), multi R x x 
   | multi_step : forall (x y z : X), R x y -> multi R y z -> multi R x z.
-
-Definition alpha_multistep : relation process := multi alphaP.
-
-End alphaP.
-
+  
 Lemma transitive_multi {X : Type} : forall (R : relation X) (x y z : X), multi R x y -> multi R y z -> multi R x z.
 Proof.
   intros R x y z H.
@@ -300,24 +796,61 @@ Proof.
   apply H2 with (y := y). easy. easy.
 Qed.
 
+Definition alpha_multistep : relation process := multi alphaP.
 
-Definition quaternary_relation (A : Type) : Type := A -> A -> A -> A -> Prop.
 
-Print relation.
-Print quaternary_relation.
+End alphaP.
+
+
+Section substitution.
+
+Definition quaternary_relation (A : Type) : Type := fin -> A -> A -> A -> Prop.
 
 (* relation of sub_from, sub_to, proc_before_sub, proc_after_sub, rec case, ensures is fresh in both x and P *)
 Inductive substitutionP : quaternary_relation process :=
-  | sub_var_is   : forall P x, substitutionP (p_var x) P (p_var x) P
-  | sub_var_not  : forall P x y, x <> y -> substitutionP (p_var x) P (p_var y) (p_var y)
-  | sub_inact    : forall P x, substitutionP (p_var x) P (p_inact) (p_inact)
-  | sub_send     : forall P x pt l e P' Q', substitutionP (p_var x) P P' Q' -> substitutionP (p_var x) P (p_send pt l e P') (p_send pt l e Q')
-  | sub_recv     : forall P x pt lb ct1 ct2 llb xs ys, length xs = length ys -> substitutionP (p_var x) P ct1 ct2 ->
-  List.Forall (fun u => substitutionP (p_var x) P (fst u) (snd u)) (zip xs ys) -> substitutionP (p_var x) P (p_recv pt lb ct1 llb xs) (p_recv pt lb ct2 llb ys)
-  | sub_ite       : forall P x e P1 P2 Q1 Q2, substitutionP (p_var x) P P1 Q1 -> substitutionP (p_var x) P P2 Q2 -> substitutionP (p_var x) P (p_ite e P1 P2) (p_ite e Q1 Q2)
-  | sub_rec       : forall P x y P' Q', x <> y -> fresh_in y P -> substitutionP (p_var x) P P' Q' -> substitutionP (p_var x) P (p_rec y P') (p_rec y Q')
-  | sub_alpha     : forall P x P1 P2 Q, alpha_multistep P1 P2 -> substitutionP (p_var x) P P1 Q -> substitutionP (p_var x) P P2 Q.
+  | sub_var_is   : forall P x,             substitutionP x P (p_var x) P
+  | sub_var_not  : forall P x y, x <> y -> substitutionP x P (p_var y) (p_var y)
+  | sub_inact    : forall P x,             substitutionP x P (p_inact) (p_inact)
+  | sub_send     : forall P x pt l e P' Q', substitutionP x P P' Q' -> substitutionP x P (p_send pt l e P') (p_send pt l e Q')
+  | sub_recv     : forall P x pt llb xs ys, length llb = length xs -> length llb = length ys -> SSortedNList llb -> 
+  List.Forall2 (substitutionP x P) xs ys -> substitutionP x P (p_recv pt llb xs) (p_recv pt llb ys)
+  | sub_ite       : forall P x e P1 P2 Q1 Q2, substitutionP x P P1 Q1 -> substitutionP x P P2 Q2 -> substitutionP x P (p_ite e P1 P2) (p_ite e Q1 Q2)
+  | sub_rec       : forall P x y P' Q', x <> y -> fresh_in y P -> substitutionP x P P' Q' -> substitutionP x P (p_rec y P') (p_rec y Q')
+  | sub_alpha     : forall P x P1 P2 Q1 Q2, alphaP P1 P2 -> alphaP Q1 Q2 -> substitutionP x P P1 Q1 -> substitutionP x P P2 Q2.
  (* | sub_alpha     : forall P x P' Q1 Q2, substitutionP (p_var x) P P' Q1 -> alphaP Q1 Q2 -> substitutionP (p_var x) P P' Q2. *)
+
+
+Section substitutionP_ind_ref.
+  
+  Variable P : fin -> process -> process -> process -> Prop.
+  Hypothesis P_var_is : forall Pr X, P X Pr (p_var X) Pr.
+  Hypothesis P_var_not : forall Pr X Y, X <> Y -> P X Pr (p_var Y) (p_var Y).
+  Hypothesis P_inact : forall Pr X, P X Pr p_inact p_inact.
+  Hypothesis P_send : forall Pr X pt l e P' Q', P X Pr P' Q' -> P X Pr (p_send pt l e P') (p_send pt l e Q').
+  Hypothesis P_recv : forall Pr X pt llb xs ys, length llb = length xs -> length llb = length ys -> SSortedNList llb 
+                              -> List.Forall2 (P X Pr) xs ys -> P X Pr (p_recv pt llb xs) (p_recv pt llb ys).
+  Hypothesis P_ite : forall Pr X e P1 P2 Q1 Q2, P X Pr P1 Q1 -> P X Pr P2 Q2 -> P X Pr (p_ite e P1 P2) (p_ite e Q1 Q2).
+  Hypothesis P_rec : forall Pr X Y P1 Q1, X <> Y -> fresh_in Y Pr -> P X Pr P1 Q1 -> P X Pr (p_rec Y P1) (p_rec Y Q1).
+  Hypothesis P_alpha : forall Pr X P1 P2 Q1 Q2, alphaP P1 P2 -> alphaP Q1 Q2 -> P X Pr P1 Q1 -> P X Pr P2 Q2.
+  
+  Fixpoint substitutionP_ind_ref (X : fin) (Pr P1 P2 : process) (a : substitutionP X Pr P1 P2) {struct a} : P X Pr P1 P2 :=
+    match a with 
+      | sub_var_is p x => P_var_is p x
+      | sub_var_not p x y Hn => P_var_not p x y Hn
+      | sub_inact p x => P_inact p x
+      | sub_send p x pt l e P' Q' H => P_send p x pt l e P' Q' (substitutionP_ind_ref x p P' Q' H)
+      | sub_recv p x pt llb xs ys Hbx Hby HSb Lxy => P_recv p x pt llb xs ys Hbx Hby HSb (Forall2_mono (substitutionP_ind_ref x p) xs ys Lxy)
+      | sub_ite p x e p1 p2 q1 q2 H1 H2 => P_ite p x e p1 p2 q1 q2 (substitutionP_ind_ref x p p1 q1 H1) (substitutionP_ind_ref x p p2 q2 H2)
+      | sub_rec p x y p1 q1 Hn Hfy Hsb => P_rec p x y p1 q1 Hn Hfy (substitutionP_ind_ref x p p1 q1 Hsb)
+      | sub_alpha p x p1 p2 q1 q2 Hap Haq Hsb => P_alpha p x p1 p2 q1 q2 Hap Haq (substitutionP_ind_ref x p p1 q1 Hsb)  
+    end.
+
+End substitutionP_ind_ref.
+
+
+
+(* Lemma inv_subst_send : forall x P Q1 Q2 P' pt l e, substitutionP x P Q1 Q2 -> (Q1 = p_send pt l e P') -> exists 
+   *)
   
 
 (* Example alpha_subst : substitutionP (p_var 0) (p_var 1) (p_rec 1 (p_ite (e_var 100) (p_var 0) (p_var 1))) (p_rec 2 (p_ite (e_var 100) (p_var 1) (p_var 2))).
@@ -406,6 +939,8 @@ Definition subst_expr_proc (p : process) (l : label) (e : expr) : (option proces
 
 
  *)
+
+End substitution.
 
 End process.
 
